verif/btrees/btrees_functional.v
@@ -1,22 +1,25 @@
-(** * btrees.v : Formal Model of BTrees  *)
-From Equations Require Import Equations.
+Require Import VST.floyd.functional_base.
 Require Import VST.floyd.proofauto.
-Require Import VST.floyd.library.
 Require Import VST.progs.conclib.
-Require Import Sorting.Sorted.
 Require Import Program.Basics. (* for compose *)
 Require Import Program.Combinators. (* for compose notation "∘" *)
 
-Import ListNotations.
+Definition param: Z := 8.
+Definition max_depth: Z := 20.
 
-Definition param: nat := 8.
-Definition max_depth: nat := 20.
+Lemma param_eq: param = 8. Proof. reflexivity. Qed.
+Lemma max_depth_eq: max_depth = 20. Proof. reflexivity. Qed.
+Opaque param. Opaque max_depth.
+
+Hint Rewrite param_eq: rep_omega. Hint Rewrite max_depth_eq: rep_omega.
 
 Definition K: Type := Z.
+
 Definition V: Type := {p: val | is_pointer_or_null p}.
 Definition nullV: V := exist _ nullval mapsto_memory_block.is_pointer_or_null_nullval.
 
 Instance Inhabitant_V: Inhabitant V := nullV.
+
 Instance EqDecV: EqDec V.
 Proof.
   intros [x hx] [y hy]. destruct (eq_dec x y) as [heq | hneq].
@@ -24,141 +27,88 @@ Proof.
   + right. intro hcontr. apply hneq. inversion hcontr. reflexivity.
 Qed.
 
-(* B+tree abtract model *)
-Inductive node: Z -> Type :=
-| leaf: forall (records: list (K * V)) (address: val), node 0
-| internal: forall {d} (ptr0: node d) (children: list (K * node d)) (address: val), node (Z.succ d).
+Unset Elimination Schemes.
+Inductive node: Type :=
+| leaf: forall (records: list (K * V)) (address: val), node
+| internal: forall (ptr0: node) (children: list (K * node)) (address: val), node.
 
-Definition is_leaf {d} (n: node d): Prop :=
+Inductive balanced: Z -> node -> Prop :=
+| balanced_leaf: forall {l p}, balanced 0 (leaf l p)
+| balanced_internal: forall {d ptr0 l p}, balanced d ptr0 -> Forall (balanced d ∘ snd) l ->
+                                     balanced (Z.succ d) (internal ptr0 l p). 
+
+Instance Inhabitant_node: Inhabitant node :=
+  leaf (combine (upto (Z.to_nat param)) (Zrepeat param nullV)) nullval.
+
+Definition is_leaf (n: node): Prop :=
   match n with
   | leaf _ _ => True
   | _ => False
-end.
+  end.
 
-Definition is_leaf_dec {d} (n: node d): {is_leaf n} + {not (is_leaf n)} :=
-match n as m return {is_leaf m} + {not(is_leaf m)} with
-| leaf _ _ => left I
-| internal _ _ _ _ => right (fun hcontr => hcontr)
-end.
+Definition is_leaf_dec (n: node): {is_leaf n} + {not (is_leaf n)} :=
+  match n as m return {is_leaf m} + {not(is_leaf m)} with
+  | leaf _ _ => left I
+  | internal _ _ _ => right (fun hcontr => hcontr)
+  end.
 
-Definition keys {d} (n: node d): list K := 
+Definition keys (n: node): list K := 
   match n with
   | leaf recs _ => map fst recs
-  | internal _ _ children _ => map fst children
+  | internal _ children _ => map fst children
   end.
 
-Definition address {d} (n: node d): val := 
-  match n with | leaf _ p => p | internal _ _ _ p => p end.
+Definition node_address (n: node): val := 
+  match n with | leaf _ p => p | internal _ _ p => p end.
 
-(* number of keys in a node *)
-Definition num_keys {d} (n: node d) : Z :=
-match n with leaf l _ => Zlength l | internal _ _ l _ => Zlength l end.
+Arguments node_address n: simpl nomatch.
 
-Section node_ind.
-  Variables (P: forall d, node d -> Prop) (Q : forall d, list (K * node d) -> Prop).
+Definition num_keys (n: node): Z :=
+  match n with leaf l _ => Zlength l | internal _ l _ => Zlength l end.
 
-  Hypotheses
-    (hleaf: forall l v, P 0 (leaf l v))
-    (hinternal : forall d ptr0 (entries: list (K * node d)) v,
-        P d ptr0 -> Q d entries -> P (Z.succ d) (internal ptr0 entries v))
-    (hnil : forall d, Q d [])
-    (hcons : forall d (k: K) (n: node d), P d n -> forall l: list (K * node d), Q d l -> Q d (cons (k,n) l)).
-
-  Fixpoint general_node_ind {d} (n: node d): P d n :=
-    match n as x in node d return P d x with
-    | leaf l v => hleaf l v
-    | internal d ptr0 l v =>
-      hinternal d ptr0 l v (general_node_ind ptr0)
-                (((fix l_ind (l':list (K * node d)) : Q d l' :=
-                     match l' as x return Q d x with
-                     | nil => hnil d
-                     | cons (k1, n1) tl => hcons d k1 n1 (general_node_ind n1) tl (l_ind tl)
-                     end)) l)
-    end.
-End node_ind.
-(*
-Section node_rect.
-  Variables (P : node -> Type) (Q : list (K * node)-> Type).
-
-  Hypotheses
-    (hleaf: forall l v, P (leaf l v))
-    (hinternal : forall ptr0 (entries:list (K * node)) v,
-        P ptr0 -> Q entries -> P (internal ptr0 entries v))
-    (hnil : Q [])
-    (hcons : forall (k: K) (n: node), P n -> forall l: list (K * node), Q l -> Q (cons (k,n) l)).
-
-  Fixpoint general_node_rect (n: node): P n :=
-    match n as x return P x with
-    | leaf l v => hleaf l v
-    | internal ptr0 l v =>
-      hinternal ptr0 l v (general_node_rect ptr0)
-                (((fix l_ind (l':list (K * node)) : Q l' :=
-                     match l' as x return Q x with
-                     | nil => hnil
-                     | cons (k1, n1) tl => hcons k1 n1 (general_node_rect n1) tl (l_ind tl)
-                     end)) l)
-    end.
-End node_rect.
-*)
-
-Lemma node_ind2 (P: forall d, node d -> Prop)
-        (hleaf: forall entries val, P 0 (leaf entries val))
-        (hinternal : forall d ptr0 (entries:list (K * node d)) val,
-            P d ptr0 -> Forall (P d ∘ snd) entries -> P (Z.succ d) (internal ptr0 entries val)):
-  forall d (n: node d), P d n.
-Proof.
-  apply general_node_ind with (Q := fun d l => Forall (P d ∘ snd) l).
-  assumption. assumption. easy. now constructor.
-Qed.
-
-(*
-Definition node_rect2 (P: node -> Type)
-        (hleaf: forall entries val, P (leaf entries val))
-        (hinternal : forall ptr0 (entries:list (K * node)) val,
-            P ptr0 -> (forall e, In e entries -> P (snd e)) -> P (internal ptr0 entries val)):
-  forall n: node, P n.
-Proof.
-  refine (general_node_rect P (fun entries => forall e, In e entries -> P (snd e)) hleaf hinternal _ _).
-  easy.
-  intros k n hn l hl kn hinkn%in_inv.
-  destruct (in_dec (prod_eqdec Z.eq_dec node_eq_dec) kn l) as [h|h]. apply (hl _ h).
-  destruct (prod_eqdec Z.eq_dec node_eq_dec kn (k, n)) as [h'|h']. subst. easy.
-  exfalso. apply h. destruct hinkn. subst; contradiction. assumption.
-Qed.
-*)
-
-(* Abstracting a B+tree to an ordered list of (key,value) pairs *)
-Fixpoint abs_node {d} (n: node d) : list (K * V) :=
+(* Abstracting a node to an ordered list of (key,value) pairs *)
+Fixpoint abs_node (n: node): list (K * V) :=
   match n with
   | leaf le _ => le
-  | internal _ ptr0 le _ => abs_node ptr0 ++ flat_map (abs_node ∘ snd) le
+  | internal ptr0 le _ => abs_node ptr0 ++ flat_map (abs_node ∘ snd) le
   end.
 
-(* Number of records the B+tree is holding *)
-Fixpoint num_records {d} (n: node d): Z :=
+Fixpoint num_records (n: node): Z :=
   match n with
   | leaf le _ => Zlength le
-  | internal _ ptr0 le _ => num_records ptr0 + fold_right Z.add 0 (map (num_records ∘ snd) le)
+  | internal ptr0 le _ => num_records ptr0 + fold_right Z.add 0 (map (num_records ∘ snd) le)
   end.
 
-Lemma numrec_abs_node_length {d} (n: node d): Zlength (abs_node n) = num_records n.
+Lemma node_ind (P: node -> Prop)
+      (hleaf: forall l p, P (leaf l p))
+      (hinternal: forall ptr0 l p, P ptr0 -> Forall (P ∘ snd) l -> P (internal ptr0 l p)) : forall n, P n.
 Proof.
-  apply (node_ind2 (fun _ n => Zlength (abs_node n) = num_records n)).
+  fix hrec 1.
+  intros [].
+  apply hleaf.
+  apply hinternal. apply hrec.
+  induction children as [|[k n] children]. constructor.
+  constructor. cbn. apply hrec. assumption.
+Qed.
+
+Lemma numrec_abs_node_length n : Zlength (abs_node n) = num_records n.
+Proof.
+  apply (node_ind (fun n => Zlength (abs_node n) = num_records n)).
   + intros. reflexivity.
   + intros * hlength hforall.
     simpl. rewrite Zlength_app, hlength, flat_map_concat_map, Zlength_concat,
-    map_map. do 2 f_equal.
+           map_map. do 2 f_equal.
     apply map_ext_in.
     intros [k n']. rewrite Forall_forall in hforall.
     apply hforall.
 Qed.
 
-Inductive cursor: forall {d} (root: node d), Type :=
+Inductive cursor: forall (root: node), Type :=
 | leaf_cursor: forall {l p} (k: K) (ptr: V) (i: Z)
                  (hi: 0 <= i < Zlength l)
                  (h: Znth i l = (k, ptr)), cursor (leaf l p) 
-| ptr0_cursor: forall {d} {ptr0: node d} {l p} (tl: cursor ptr0), cursor (internal ptr0 l p)
-| le_child_cursor: forall {d ptr0 l p} (k: K) (child: node d) (i: Z)
+| ptr0_cursor: forall {ptr0: node} {l p} (tl: cursor ptr0), cursor (internal ptr0 l p)
+| le_child_cursor: forall {ptr0 l p} (k: K) (child: node) (i: Z)
                      (hi: 0 <= i < Zlength l)
-                     (h: @Znth _ (k, child) i l = (k, child))
-                  (tl: cursor child), cursor (internal ptr0 l p).
+                     (h: Znth i l = (k, child))
+                     (tl: cursor child), cursor (internal ptr0 l p).
