verif/btrees/btrees_sep.v
@@ -7,85 +7,100 @@ Require Import btrees.
 Instance CompSpecs : compspecs. make_compspecs prog. Defined.
 Definition Vprog : varspecs. mk_varspecs prog. Defined.
 
-Definition t_node := Tstruct _node noattr.
-Definition t_entry:= Tstruct _entry noattr.
-Definition t_btree := Tstruct _btree noattr.
-Definition t_cursor_entry := Tstruct _cursor_entry noattr.
-Definition t_cursor := Tstruct _cursor noattr.
+Definition tnode := Tstruct _node noattr.
+Definition tentry:= Tstruct _entry noattr.
+Definition tbtree := Tstruct _btree noattr.
+Definition tcursor_entry := Tstruct _cursor_entry noattr.
+Definition tcursor := Tstruct _cursor noattr.
 
 Require Import Program.Basics. Require Import Program.Combinators.
 
-Fixpoint node_rep {d} (n: node d): mpred :=
+Section Complete.
+
+Definition complete MAX l := l ++ repeat (Vundef, Vundef) (Z.to_nat MAX - length l).
+
+Lemma Znth_complete : forall n l MAX, n < Zlength l -> 
+     Znth n (complete MAX l) = Znth n l.
+Proof.
+  intros; apply app_Znth1; auto.
+Qed.
+
+Lemma Zlength_complete : forall l m, Zlength l <= m -> Zlength (complete m l) = m.
+Proof.
+  intros; unfold complete.
+  rewrite Zlength_app, Zlength_repeat; rewrite Zlength_correct in *; rep_omega.
+Qed.
+
+End Complete.
+
+Fixpoint node_rep (n: node): mpred :=
+malloc_token Ews tnode (node_address n) *
 match n with
 | leaf l p =>
-  EX b: val,
-  !! typed_true tuchar b &&
-  malloc_token Ews t_node p *
-  data_at Ews t_node
-          (b,
+  data_at Ews tnode
+          (Val.of_bool true,
            (vint (Zlength l),
             (Vnullptr,
-             force_lengthn (2*param+1) (map (fun '(k, ptr) => (vint k, proj1_sig ptr)) l) (Vundef, Vundef)))) p
-
-| internal _ ptr0 l p as n =>
-  EX b: val,
-  !! typed_false tuchar b &&
-  malloc_token Ews t_node p *
-  data_at Ews t_node
-          (b,
+             complete (2*param+1) (map (fun '(k, ptr) => (vint k, proj1_sig ptr)) l)))) p
+| internal ptr0 l p =>
+  data_at Ews tnode
+          (Val.of_bool false,
            (vint (Zlength l),
-            (address ptr0,
-             force_lengthn (2*param+1) (map (fun '(k, n) => (vint k, address n)) l) (Vundef, Vundef)))) p *
+            (node_address ptr0,
+             complete (2*param+1) (map (fun '(k, n) => (vint k, node_address n)) l)))) p *
   node_rep ptr0 *
   iter_sepcon (node_rep ∘ snd) l
 end.
 
-Lemma node_rep_local_facts {d} (n: node d):
-    node_rep n |-- !! isptr (address n).
+Lemma node_valid_pointer (n: node):
+    node_rep n |-- valid_pointer (node_address n).
 Proof.
-  destruct n; cbn; entailer.
-Qed.
-  
-Hint Resolve node_rep_local_facts: saturate_local.
-
-Lemma node_valid_pointer {d} (n: node d):
-    node_rep n |-- valid_pointer (address n).
-Proof.
-  destruct n; cbn; entailer.
+  destruct n;
+  unfold node_rep; fold node_rep;
+  auto with valid_pointer.
 Qed.
 
 Hint Resolve node_valid_pointer: valid_pointer.
 
-Definition btree_rep {d} (root: node d) (p: val): mpred :=
-  malloc_token Ews t_btree p
-  * data_at Ews t_btree (address root, (vint (num_records root), vint d)) p
+Lemma node_rep_local_facts (n: node):
+    node_rep n |-- !! isptr (node_address n).
+Proof.
+  destruct n; unfold node_rep; fold node_rep;
+  entailer.
+Qed.
+  
+Hint Resolve node_rep_local_facts: saturate_local.
+
+Definition btree_rep {d} (root: node) (h: balanced d root) (p: val): mpred :=
+  malloc_token Ews tbtree p
+  * data_at Ews tbtree (node_address root, (vint (num_records root), vint d)) p
   * node_rep root.
 
-Lemma btree_rep_local_facts {d} (n: node d) (p: val):
-    btree_rep n p |-- !! isptr p.
+Lemma btree_rep_local_facts {d} (n: node) (h: balanced d n) (p: val):
+    btree_rep n h p |-- !! isptr p.
 Proof.
   unfold btree_rep; entailer.
 Qed.
   
 Hint Resolve btree_rep_local_facts: saturate_local.
 
-Lemma btree_valid_pointer {d} (n: node d) (p: val):
-    btree_rep n p |-- valid_pointer p.
+Lemma btree_valid_pointer {d} (n: node) (h: balanced d n) (p: val):
+    btree_rep n h p |-- valid_pointer p.
 Proof.
   unfold btree_rep. auto with valid_pointer.
 Qed.
 
 Hint Resolve btree_valid_pointer: valid_pointer.
 
-Fixpoint cursor_entries {d} {root: node d} (c: cursor root): list (val * val) :=
+Fixpoint cursor_entries {root: node} (c: cursor root): list (val * val) :=
 match c with
 | leaf_cursor l p _ _ i _ _ => [(vint i, p)]
-| ptr0_cursor _ _ _ p c => (vint (-1), p) :: cursor_entries c
-| le_child_cursor _ _ _ p _ _ i _ _ c => (vint i, p) :: cursor_entries c
+| ptr0_cursor _ _ p c => (vint (-1), p) :: cursor_entries c
+| le_child_cursor _ _ p _ _ i _ _ c => (vint i, p) :: cursor_entries c
 end.
 
 (* Several cursors can point to the same btree structure. *)
-Definition cursor_rep {d} {root: node d} (c: cursor root) (p: val): mpred :=
+Definition cursor_rep {root: node} (level: Z) (c: cursor root) (p: val): mpred :=
   EX ptree: val,
-  data_at Ews t_cursor (ptree, (vint d,
-                                force_lengthn max_depth (cursor_entries c) (Vundef, Vundef))) p.
+  data_at Ews tcursor (ptree, (vint level,
+                                force_lengthn (Z.to_nat max_depth) (cursor_entries c) (Vundef, Vundef))) p.
