verif/btrees/btrees_spec.v
@@ -16,49 +16,99 @@ Definition new_btree_spec : ident * funspec :=
          PROP ()
          LOCAL (gvars gv)
          SEP (mem_mgr gv)
-  POST [ tptr t_btree ]
+  POST [ tptr tbtree ]
     EX p:val, EX p_root: val,
          PROP ()
          LOCAL (temp ret_temp p)
-         SEP (mem_mgr gv; btree_rep (leaf [] p_root) p).
+         SEP (mem_mgr gv; btree_rep (leaf [] p_root) balanced_leaf p).
+
+Definition ptr_at_spec : ident * funspec :=
+  DECLARE _ptr_at
+  WITH gv: globals, n: node, i: Z
+  PRE [ _n OF tptr tnode, _i OF tint ]
+         PROP (Int.min_signed <= i <= Int.max_signed; i < num_keys n <= 2*param)
+         LOCAL (gvars gv; temp _n (node_address n); temp _i (vint i))
+         SEP (mem_mgr gv; node_rep n)
+  POST [ tptr tvoid ]
+  let res :=
+  match n with
+  | leaf l p => proj1_sig (snd (Znth i l))
+  | internal ptr0 l p => if i <? 0 then node_address ptr0 else node_address (snd (Znth i l))
+  end in
+         PROP ()
+         LOCAL (temp ret_temp res)
+         SEP (mem_mgr gv; node_rep n).
 
 Definition Gprog : funspecs :=
         ltac:(with_library prog [ new_btree_spec ]).
 
-Set Default Timeout 30.
+Set Default Timeout 20.
+Arguments proj_reptype _ _ _ v: simpl never.
+Arguments force_lengthn A n xs default: simpl never.
+
+Lemma body_ptr_at: semax_body Vprog Gprog f_ptr_at ptr_at_spec.
+Proof.
+  start_function.
+  forward_if.
+  + destruct n; unfold node_address, node_rep; fold node_rep;
+    Intros; do 2 forward.
+    { apply prop_right. rewrite Znth_underflow. reflexivity. rep_omega. }
+    { entailer!. rewrite Zaux.Zlt_bool_true by assumption. reflexivity.
+    unfold node_rep; fold node_rep. entailer!. }
+  + forward_if.
+    - forward.
+    - destruct n; unfold node_address, node_rep; fold node_rep;
+      Intros.
+      { assert (h: snd (Znth i (complete 17 (map (fun '(k, ptr) => (vint k, proj1_sig ptr)) records))) = proj1_sig (snd (Znth i records))).
+        { simpl in H0. destruct H0.
+          rewrite Znth_complete, Znth_map by
+          (try rewrite Zlength_map; fold K V; rep_omega).  now destruct Znth. }
+        forward. entailer!. setoid_rewrite h. now destruct (snd (Znth i records)).
+        forward. }
+      { simpl in H0. destruct H0.
+        assert (h: snd (Znth i (complete 17 (map (fun '(k, ptr) => (vint k, node_address ptr)) children))) = node_address (snd (Znth i children))).
+        { rewrite Znth_complete, Znth_map by
+              (try rewrite Zlength_map; fold K V; rep_omega).  now destruct Znth. }
+        forward. entailer. setoid_rewrite h.
+        rewrite iter_sepcon_Znth with (i0 := i) by rep_omega. cbn. entailer.
+        forward.
+        setoid_rewrite h. rewrite Zaux.Zlt_bool_false by omega. cbn.
+        entailer!.
+      }
+Qed.
+
 
 Lemma body_new_btree: semax_body Vprog Gprog f_new_btree new_btree_spec.
 Proof.
   start_function.
-  forward_call (t_btree, gv).
+  forward_call (tbtree, gv).
   easy.
   Intro p.
   forward.
   forward_if
     (PROP ( )
      LOCAL (temp _t p; temp _t'2 p; gvars gv)
-     SEP (mem_mgr gv; malloc_token Ews t_btree p; data_at_ Ews t_btree p)).
+     SEP (mem_mgr gv; malloc_token Ews tbtree p; data_at_ Ews tbtree p)).
   + destruct eq_dec; entailer!.
   + subst. rewrite eq_dec_refl. forward_call tt. contradiction.
   + rewrite if_false by assumption.
     forward.
     entailer!.
-  + forward_call (t_node, gv).
+  + forward_call (tnode, gv).
     easy.
-    Intro p_root.
-    forward. simpl.
+    Intros p_root.
+    forward.
     forward_if
      (PROP ( )
      LOCAL (temp _t'4 p_root; temp _t p; temp _t'2 p; gvars gv)
-     SEP (mem_mgr gv; malloc_token Ews t_node p_root; data_at_ Ews t_node p_root;
-     malloc_token Ews t_btree p; data_at Ews t_btree (p_root, (Vundef, Vundef)) p)).
+     SEP (mem_mgr gv; malloc_token Ews tnode p_root; data_at_ Ews tnode p_root;
+     malloc_token Ews tbtree p; data_at Ews tbtree (p_root, (Vundef, Vundef)) p)).
   - destruct eq_dec; entailer.
   - subst; rewrite eq_dec_refl. forward_call tt. contradiction.
   - rewrite if_false by assumption.
     forward. entailer!.
   - do 9 forward.
-    unfold btree_rep, node_rep.
-    Exists p p_root (Vint (Int.zero_ext 8 (Int.repr 1))).
-    change Vnullptr with (vint 0). entailer.
-    simpl. rewrite Zlength_nil. simpl nested_field_type. simpl nested_field_offset. cancel.
+    unfold btree_rep, node_rep, node_address. 
+    Exists p p_root.
+    entailer!.
 Qed.
